Definition -> Lemma

theories/base_logic/lib/fancy_updates.v
@@ -12,7 +12,7 @@ Definition uPred_fupd_def `{!invG Σ} (E1 E2 : coPset) (P : iProp Σ) : iProp Σ
 Definition uPred_fupd_aux : seal (@uPred_fupd_def). Proof. by eexists. Qed.
 Definition uPred_fupd := uPred_fupd_aux.(unseal).
 Arguments uPred_fupd {Σ _}.
-Definition uPred_fupd_eq `{!invG Σ} : @fupd _ uPred_fupd = uPred_fupd_def.
+Lemma uPred_fupd_eq `{!invG Σ} : @fupd _ uPred_fupd = uPred_fupd_def.
 Proof. rewrite -uPred_fupd_aux.(seal_eq) //. Qed.
 
 Lemma uPred_fupd_mixin `{!invG Σ} : BiFUpdMixin (uPredI (iResUR Σ)) uPred_fupd.
